\documentclass[sectionformat=aufgabe]{gadsescript}

\setsemester{Summer Semester 2024}%
\setuniversity{University of Konstanz}%
\settitlelh{\today\\\semester\\Gruppe 3, Jonathan Weihing}
\setfaculty{Faculty of Science\\(Mathematics and Statistics)}%
\settitle{Übungsblatt 7}
\setsubtitle{Elias Gestrich}
\usepackage{subfig}

\begin{document}
\maketitle
\begin{align*}
	\partial_i \left\| x \right\| &= \partial_i \left( \sum_{i=1}^{n} x_i^2 \right) ^{\frac{ 1 }{ 2 } }   \\
	~ &= \left( 2 x_i \right) \cdot \frac{ 1 }{ 2 } \left( \sum_{i=1}^{n} x_i^2 \right) ^{-\frac{ 1 }{ 2 } }   \\
	~ &= \frac{ \left( x_i \right) }{ \left\| x \right\| }   \\
\end{align*}

\begin{align*}
	\partial_i \left\| x \right\|^2 &= \partial_i \left( \left(\sum_{i=1}^{n} x_i^2\right)^{\frac{ 1 }{ 2 } } \right) ^2 \\
	\partial_i \left\| x \right\|^2 &= \partial_i \sum_{i=1}^{n} x_i^2 \\
	~ &= \left( 2 x_i \right)  \\
\end{align*}

\section{Wärmeleitungskern}
\begin{align*}
	\Delta F &= \sum_{i=1}^{n} \partial_i^2 F \\
	~ &= \sum_{i=1}^{n} \partial_i^2 t^{- \frac{ n }{ 2 } } \exp \left( - \frac{ \left\| x \right\| ^2 }{ 4t }  \right)  \\
	~ &= \sum_{i=1}^{n} \partial_i - \frac{2 x_i}{ 4t }  t ^{- \frac{ n }{ 2 } } \exp \left( - \frac{ \left\| x \right\| ^2 }{ 4t }  \right)  \\
	~ &= \sum_{i=1}^{n}
	\left( - \frac{ 2 }{ 4t } t ^{- \frac{ n }{ 2 } } \exp \left( - \frac{ \left\| x \right\| ^2 }{ 4t }  \right)  \right)
	+
	\left( \frac{ 4x_i^2 }{ 16t^2 } t ^{- \frac{ n }{ 2 } } \exp \left( - \frac{ \left\| x \right\| ^2 }{ 4t }  \right)   \right)  \\
	~ &= \left( - \frac{ 1 }{ 2 } t ^{- \frac{ n }{ 2 } - 1 } \exp \left( - \frac{ \left\| x \right\| ^2 }{ 4t }  \right)  \right) \left( \sum_{i=1}^{n} 1 \right) 
	+
	\left( \frac{ 1 }{ 4 } t ^{- \frac{ n }{ 2 } - 2 } \exp \left( - \frac{ \left\| x \right\| ^2 }{ 4t }  \right)   \right) \sum_{i=1}^{n} x_i^2 \\
	~ &= \left( - \frac{ n }{ 2 } t ^{- \frac{ n }{ 2 } - 1 } \exp \left( - \frac{ \left\| x \right\| ^2 }{ 4t }  \right)  \right) 
	+
	\left( \frac{ \left\| x \right\| ^2 }{ 4 } t ^{- \frac{ n }{ 2 } - 2 } \exp \left( - \frac{ \left\| x \right\| ^2 }{ 4t }  \right)   \right) \\
	~ &= \left( \frac{ \left\| x \right\| ^2 t ^{-\frac{ n }{ 2 } - 2} }{ 4 } - \frac{ n t ^{-\frac{ n }{ 2 } -1} }{ 2 }  \right) \exp \left( - \frac{ \left\| x \right\| ^2 }{ 4t }  \right)  \\
\end{align*}
und
\begin{align*}
	\frac{ \partial F }{ \partial t } &= \left( - \frac{ n }{ 2 } t ^{-\frac{ n }{ 2 } -1} \exp \left( - \frac{ \left\| x \right\| ^2 }{ 4t }  \right) \right) - \left( \left(- \frac{ \left\| x \right\| ^2 }{ 4t^2 } \right) t^{-\frac{ n }{ 2 } } \exp \left( - \frac{\left\| x \right\| ^2 }{ 4t }  \right)  \right) \\
	~ &= \left( \frac{ \left\| x \right\| ^2 t ^{-\frac{ n }{ 2 } - 2} }{ 4 } - \frac{ n t ^{-\frac{ n }{ 2 } -1} }{ 2 }  \right) \exp \left( - \frac{ \left\| x \right\| ^2 }{ 4t }  \right)  \\
\end{align*}

also $ \Delta F = \frac{ \partial F }{ \partial t }  $, also $ \Delta F - \frac{ \partial F }{ \partial t } = 0 $

\section{Harmonische Funktionen}
Für $ n = 2 $:
\[
	\sum_{i=1}^{2} \partial_i^2 \ln \left| x \right|
	= \sum_{i=1}^{2} \partial_i \frac{ x_i }{ \left| x \right|  } \cdot \frac{ 1 }{ \left| x \right|  }
	= \sum_{i=1}^{2} \partial_i \frac{x_i}{ \left| x \right| ^{2} }
	= \sum_{i=1}^{2} \frac{1 \cdot \left| x \right| ^2 - x_i \cdot 2 x_i }{ \left| x \right| ^{4} }
	= \frac{2 \cdot \left| x \right| ^2 - 2 \left| x \right| ^2}{ \left| x \right| ^{4} }
	= 0
\]

Für $ n > 2 $ 
\begin{align*}
	\sum_{i=1}^{n} \partial_i^2 \left| x \right| ^{2 - n}
	& = \sum_{i=1}^{n} \partial_i \frac{ x_i }{ \left| x \right|  } \left| x \right| ^{1 - n} \\
	& = \sum_{i=1}^{n} \partial_i \frac{ x_i }{ \left| x \right|^{n} } \\
	& = \sum_{i=1}^{n} \frac{ \left| x \right| ^n - x_i \cdot \frac{x_i}{ \left| x \right|  } \cdot n \left| x \right| ^{n - 1}  }{ \left| x \right|^{2n} } \\
	& = \sum_{i=1}^{n} \frac{ \left| x \right| ^n - n x_i^2 \left| x \right| ^{n - 2}  }{ \left| x \right|^{2n} } \\
	& = \frac{ n \left| x \right| ^n - n \left| x \right| ^2 \left| x \right| ^{n - 2}  }{ \left| x \right|^{2n} } \\
	& = \frac{ n \left| x \right| ^n - n \left| x \right| ^{n}  }{ \left| x \right|^{2n} } \\
	& = 0
\end{align*}

\end{document}

